yeah

SetTheory/FunctionsRelations.lean
@@ -80,13 +80,183 @@ theorem union_ordered_pair {a b: set}: (⋃ ⟪a,b⟫) =(pair a b : set) := by
       simp only [h, ordered_pair._eq_1, pair_eq_singleton_iff, singleton_eq_pair_iff, and_self]
     · exact Or.inl h
 
--- TODO def converse (a: set): set := replacement (fun a )
+@[simp] theorem exists_eq_right' {α : Sort u_1} {p : α → Prop} {a' : α} : (∃ (a : α), p a ∧  a' = a) ↔ p a' := by
+  constructor
+  · rintro ⟨a, h, rfl⟩
+    exact h
+  · intro h
+    exists a'
+
+noncomputable def converse (a: set): set := replacement (fun a => ⟪proj2 a, proj1 a⟫) (separation (fun a => ∃x y, a = ⟪x,y⟫) a)
+theorem mem_converse_iff {a x: set}: x ∈ converse a ↔ ∃y z, ⟪y,z⟫ ∈ a ∧ x = ⟪z,y⟫ := by
+  simp[converse]
+  apply Iff.intro
+  · rintro ⟨p, ⟨⟨hp, ⟨x,y,rfl⟩⟩, rfl⟩⟩
+    exists x, y
+    simp only [proj2_ordered_pair, proj1_ordered_pair, and_self, hp]
+  · rintro ⟨y, z, h, rfl⟩
+    exists ⟪y, z⟫
+    simp only [h, ordered_pair_inj, exists_and_left, exists_eq', and_true, and_self,
+      proj2_ordered_pair, proj1_ordered_pair]
+
+@[simp] theorem ordered_pair_mem_converse_iff {a x y: set}: ⟪x,y⟫ ∈ converse a ↔ ⟪y,x⟫ ∈ a := by
+  simp only [mem_converse_iff, ordered_pair_inj]
+  apply Iff.intro
+  · rintro ⟨y1,z1, hin, rfl, rfl⟩
+    exact hin
+  · intro h
+    exists y,x
+
+theorem converse_converse_subset {a: set}: converse (converse a) ⊆ a := by
+  intro x hx
+  simp only [mem_converse_iff, ordered_pair_inj] at hx
+  rcases hx with ⟨y,z,⟨_,_,h,rfl,rfl⟩,rfl⟩
+  exact h
 
 def is_relation (a: set) := ∀b ∈ a, ∃x, ∃y, b = ordered_pair x y
+
+@[simp] theorem converse_converse_eq_iff {a: set}: converse (converse a) = a ↔ is_relation a := by
+  constructor
+  · rintro h
+    rw[←h]
+    intro b hb
+    simp only [mem_converse_iff, ordered_pair_inj] at hb
+    rcases hb with ⟨y,z,_,h2⟩
+    exists z, y
+  · intro h
+    ext x
+    simp only [mem_converse_iff, ordered_pair_inj]
+    constructor
+    · rintro ⟨y,z, ⟨_,_,ha,rfl,rfl⟩, rfl⟩
+      exact ha
+    · intro xa
+      obtain ⟨y,z,rfl⟩ := h x xa
+      exists z, y, ⟨y,z,xa,rfl,rfl⟩
+
+@[simp] theorem converse_is_relation {a: set}: is_relation (converse a) := by
+  intro x
+  simp only [mem_converse_iff, forall_exists_index, and_imp]
+  rintro y z _ rfl
+  exists z, y
+
+@[simp] theorem cartesian_product_is_relation {a b: set}: is_relation (a × b) := by
+  intro x
+  simp only [mem_cartesian_product_iff, forall_exists_index, and_imp]
+  rintro y _ z _ rfl
+  exists y, z
+
+@[simp] theorem empty_set_is_relation: is_relation (∅: set) := by
+  intro x
+  simp only [mem_empty_iff, false_implies]
+
+@[simp] theorem set_union_is_relation {a: set} (h: ∀x ∈ a, is_relation x): is_relation (⋃ a) := by
+  intro x
+  simp only [mem_set_union_iff', forall_exists_index, and_imp]
+  intro y hy hx
+  exact h y hy x hx
+
+@[simp] theorem union_is_relation {a b: set} (h: is_relation a) (h2: is_relation b): is_relation (a ∪ b) := by
+  apply set_union_is_relation
+  intro x2
+  simp
+  rintro (rfl|rfl)
+  · exact h
+  · exact h2
+
+@[simp] theorem singleton_ordered_pair_is_relation {x y: set}: is_relation ({⟪x,y⟫} :set) := by
+  intro a
+  rw[mem_singleton_iff]
+  rintro rfl
+  exists x,y
+
+@[simp] theorem pair_ordered_pair_is_relation {x y v w: set}: is_relation (pair ⟪x,y⟫ ⟪v,w⟫) := by
+  intro a
+  rw[mem_pair_iff]
+  rintro (rfl|rfl)
+  · exists x,y
+  · exists v,w
+
+
+theorem subset_is_relation {a b: set} (h: is_relation a) (h2: b ⊆ a): is_relation b :=
+  fun x hx => h x (h2 _ hx)
+
+@[simp] theorem inter_is_relation_left {a b: set} (h: is_relation a): is_relation (a ∩ b) := subset_is_relation h left_inter_subset
+@[simp] theorem inter_is_relation_right {a b: set} (h: is_relation a): is_relation (b ∩ a) := subset_is_relation h right_inter_subset
+
+theorem relation_ext {a b: set} (ha: is_relation a) (hb: is_relation b) (h: ∀x y, ⟪x,y⟫ ∈ a ↔ ⟪x,y⟫ ∈ b) : a = b := by
+  ext x
+  constructor
+  · intro hx
+    obtain ⟨x,y,rfl⟩ := ha x hx
+    exact (h x y).mp hx
+  · intro hy
+    obtain ⟨x,y,rfl⟩ := hb x hy
+    exact (h x y).mpr hy
+
+theorem relation_subset_from {a b: set} (ha: is_relation a) (h: ∀x y, ⟪x,y⟫ ∈ a → ⟪x,y⟫ ∈ b) : a ⊆ b := by
+  intro x hx
+  obtain ⟨x,y,rfl⟩ := ha x hx
+  exact h x y hx
+
+@[simp] theorem converse_empty_set: converse (∅: set) = ∅ := by
+  apply relation_ext converse_is_relation empty_set_is_relation
+  intro x y
+  simp only [ordered_pair_mem_converse_iff, mem_empty_iff]
+
+@[simp] theorem converse_cartesian_product {a b: set}: converse (a × b : set) = (b × a :set) := by
+  apply relation_ext converse_is_relation cartesian_product_is_relation
+  intro x y
+  simp only [ordered_pair_mem_converse_iff, ordered_pair_mem_cartesian_product_iff]
+  exact and_comm
+
+@[simp] theorem converse_subset {a b: set} (h: a ⊆ b): converse a ⊆ converse b := by
+  apply relation_subset_from converse_is_relation
+  intro x y
+  simp only [ordered_pair_mem_converse_iff]
+  apply h
+
+theorem converse_inter {a b: set}: converse (a ∩ b) = converse a ∩ converse b := by
+  apply relation_ext converse_is_relation (inter_is_relation_left converse_is_relation)
+  intro x y
+  simp only [ordered_pair_mem_converse_iff, mem_inter_iff]
+
+@[simp] theorem for_all_mem_replacement_iff {a: set} {f: set → set} {p: set → Prop}: (∀x ∈ replacement f a, p x) ↔ (∀x ∈ a, p (f x)) := by
+  constructor
+  · intro h x ax
+    apply h (f x)
+    rw [mem_replacement_iff']
+    exists x
+  · intro h x hx
+    rw [mem_replacement_iff'] at hx
+    rcases hx with ⟨y, hy, rfl⟩
+    exact h y hy
+
+theorem converse_set_union {a: set}: converse (⋃ a) = ⋃ (replacement converse a) := by
+  apply relation_ext converse_is_relation
+  · apply set_union_is_relation
+    apply (for_all_mem_replacement_iff (a := a) (f := converse) (p := is_relation)).mpr
+    simp only [converse_is_relation, forall_const, implies_true]
+  · intro x y
+    simp only [ordered_pair_mem_converse_iff, mem_set_union_iff', mem_replacement_iff']
+    constructor
+    · rintro ⟨p,h1,h2⟩
+      exists converse p
+      exact ⟨⟨p,h1,rfl⟩, by simp only [ordered_pair_mem_converse_iff, h2]⟩
+    · rintro ⟨p, ⟨q, h, rfl⟩, h2⟩
+      exists q, h
+      simp only [ordered_pair_mem_converse_iff] at h2
+      exact h2
+
+theorem converse_union {a b: set}: converse (a ∪ b) = converse a ∪ converse b := by
+  apply relation_ext converse_is_relation (union_is_relation converse_is_relation converse_is_relation)
+  intro x y
+  simp only [ordered_pair_mem_converse_iff, mem_union_iff]
+
+
 def is_single_valued (a: set) := ∀x y z, ⟪x,y⟫ ∈ a → ⟪x,z⟫ ∈ a → y = z
---TODO def is_one_to_one
+def is_one_to_one (a: set) := is_single_valued a ∧ is_single_valued (converse a)
 def is_function (a: set) := is_relation a ∧ is_single_valued a
---TODO def is_one_to_one_function
+def is_one_to_one_function (a: set) := is_function a ∧ is_one_to_one a
 def domain (a: set) := separation (fun x => ∃ y, ⟪x,y⟫ ∈ a) (⋃ ⋃ a)
 def range (a: set) := separation (fun y => ∃ x, ⟪x,y⟫ ∈ a) (⋃ ⋃ a)
 
@@ -100,6 +270,68 @@ def range (a: set) := separation (fun y => ∃ x, ⟪x,y⟫ ∈ a) (⋃ ⋃ a)
     apply And.intro hy
     simp only [mem_ordered_pair_iff, singleton_eq_pair_iff, true_and, true_or]
   · simp only [mem_singleton_iff]
+
+@[simp] theorem mem_range_iff {a y: set}: y ∈ range a ↔ ∃x, ⟪x,y⟫ ∈ a := by
+  simp only [range, mem_separation_iff', mem_set_union_iff', and_iff_right_iff_imp,
+    forall_exists_index]
+  intro x hx
+  exists pair x y
+  apply And.intro
+  · exists ⟪x,y⟫
+    apply And.intro hx
+    simp only [ordered_pair, mem_pair_iff', pair_eq_singleton_iff, true_and, or_true]
+  · simp only [mem_pair_iff', or_true]
+
+def restrict_left (a b: set) := a ∩ (b × range a)
+
+theorem mem_restrict_left_iff {x a b: set}: x ∈ restrict_left a b ↔ x ∈ a ∧ ∃y ∈ b, ∃z, x = ⟪y,z⟫ := by
+  simp only [restrict_left, mem_inter_iff, mem_cartesian_product_iff, mem_range_iff,
+    and_congr_right_iff]
+  intro h
+  apply Iff.intro
+  · rintro ⟨y, h1, z, ⟨⟨_, _⟩, rfl⟩⟩
+    exists y
+    simp only [ordered_pair_inj, true_and, exists_eq', and_self, h1]
+  · rintro ⟨y, hy, z, rfl⟩
+    exists y
+    simp only [ordered_pair_inj, true_and, hy]
+    exists z
+    exact ⟨⟨y, h⟩, rfl⟩
+
+@[simp] theorem ordered_pair_mem_restrict_left_iff {x y a b: set}: ⟪x,y⟫ ∈ restrict_left a b ↔ (⟪x,y⟫ ∈ a ∧ x ∈ b) := by
+  simp only [mem_restrict_left_iff, ordered_pair_inj, exists_and_left, exists_eq', and_true,
+    exists_eq_right']
+
+infixr:50 "↾"  => restrict_left
+def image (a b: set) := range (restrict_left a b)
+
+@[simp] theorem mem_image_iff {x a b: set}: x ∈ image a b ↔ ∃y ∈ b, ⟪y,x⟫ ∈ a := by
+  simp only [image, mem_range_iff, ordered_pair_mem_restrict_left_iff]
+  exact exists_congr $ fun y => and_comm
+
+infixr:45 "“" => image
+
+def comp (a b: set) := separation (fun p => ∃x, ∃y, ∃ z, p = ⟪x,y⟫ ∧ ⟪x,z⟫ ∈ b ∧ ⟪z,y⟫ ∈ a) (domain b × range a)
+theorem mem_comp_iff {x a b: set}: x ∈ comp a b ↔ ∃w, ∃y, ∃ z, x = ⟪w,y⟫ ∧ ⟪w,z⟫ ∈ b ∧ ⟪z,y⟫ ∈ a := by
+  simp only [comp, exists_and_left, mem_separation_iff', and_iff_right_iff_imp, forall_exists_index,
+    and_imp]
+  rintro y z rfl w yw wz
+  simp only [ordered_pair_mem_cartesian_product_iff, mem_domain_iff, mem_range_iff]
+  exact ⟨⟨w,yw⟩,⟨w,wz⟩⟩
+
+@[simp] theorem ordered_pair_mem_comp_iff {x y a b: set}: ⟪x,y⟫ ∈ comp a b ↔ ∃z, ⟪x,z⟫ ∈ b ∧ ⟪z,y⟫ ∈ a := by
+  simp only [mem_comp_iff, ordered_pair_inj, exists_and_left]
+  constructor
+  · rintro ⟨_,_,⟨rfl,rfl⟩,w,⟨h1,h2⟩⟩
+    exists w
+  · rintro ⟨z,hb,ha⟩
+    exists x,y,⟨rfl,rfl⟩,z
+
+infixr:90 " ∘ "  => comp
+
+theorem mem_comp_from_mem_rels {x y z a b: set} (h: ⟪z,y⟫ ∈ a) (h2: ⟪x,z⟫ ∈ b): ⟪x,y⟫ ∈ comp a b := by
+  rw[ordered_pair_mem_comp_iff]
+  exists z
 
 
 end ZFC
