SetTheory.lean
@@ -1,1 +1,2 @@
-def hello := "world"
+import SetTheory.Basic
+import SetTheory.FunctionsRelations
