lakefile.lean
@@ -1,6 +1,6 @@
 import Lake
 open Lake DSL
-require std from git "https://github.com/leanprover/std4" @ "main"
+require std from git "https://github.com/leanprover/std4" @ "nightly-testing"
 
 package «SetTheory» {
   --leanOptions := []  -- add package configuration options here
